theories/Decidability/Completeness.v
@@ -14,6 +14,7 @@ Import IndexedDefinitions.
 
 Equations Derive NoConfusion Subterm for term.
 
+
 Section RedImplemComplete.
 
   #[local]Definition R_aux := lexprod term term cored term_subterm.
@@ -337,6 +338,21 @@ Proof.
     reflexivity.
 Qed.
 
+Arguments PFun_instance_1 : simpl never.
+
+
+(* The combinator rec throws in a return branch with a type 
+  necessarily convertible to the result type, but the syntactic 
+  mismatch between the 2 types prevents `rec_graph` from `apply`ing.
+  This tactic fixes the type in the return branch to what's expected
+  syntactically. *)
+Ltac patch_rec_ret :=
+  try (unfold rec;
+  match goal with 
+  | |- orec_graph _ (_rec _ (fun _ : ?Bx => _)) ?hBa => 
+    let Ba := type of hBa in change Bx with Ba
+  end).
+
 Lemma implem_conv_complete :
   BundledConvInductionConcl PTyEq PTyRedEq PNeEq PNeRedEq PTmEq PTmRedEq.
 Proof.
@@ -357,9 +373,8 @@ Proof.
   - intros * HA [IHA] HB [IHB] ** ; cbn in *.
     unfold graph.
     simp conv conv_ty_red ; cbn.
-    repeat (match goal with |- orec_graph _ _ _ => econstructor end) ; cbn.
-    1: exact (IHA tt).
-    econstructor.
+    econstructor.  1: exact (IHA tt).
+    cbn; patch_rec_ret; econstructor.
     1: exact (IHB tt).
     now econstructor.
   - intros ; cbn in *.
@@ -377,9 +392,9 @@ Proof.
   - intros * HA [IHA] HB [IHB] **; cbn in *.
     unfold graph.
     simp conv conv_ty_red ; cbn.
-    repeat (match goal with |- orec_graph _ _ _ => econstructor end) ; cbn.
-    1: exact (IHA tt).
     econstructor.
+    1: exact (IHA tt).
+    cbn; patch_rec_ret; econstructor.
     1: exact (IHB tt).
     now econstructor.
   - intros * HM [IHM []] **.
@@ -463,7 +478,7 @@ Proof.
     simp conv conv_tm_red ; cbn.
     econstructor.
     1: exact IHA.
-    econstructor.
+    cbn; patch_rec_ret; econstructor.
     1: exact IHB.
     now constructor.
   - intros.
@@ -477,8 +492,7 @@ Proof.
   - intros * ? [IHt] **.
     unfold graph.
     simp conv conv_tm_red; cbn.
-    (* change (conv_full_cod (tm_state; Γ; tNat; t; t')) with (conv_full_cod (tm_red_state; Γ; tNat; tSucc t; tSucc t')). *)
-    econstructor.
+    patch_rec_ret; econstructor.
     1: exact IHt.
     now constructor.
   - intros.
@@ -488,7 +502,7 @@ Proof.
   - intros * ?? ? [IHf] **.
     unfold graph.
     simp conv conv_tm_red ; cbn.
-    econstructor.
+    patch_rec_ret; econstructor.
     1: exact IHf.
     now constructor.
   - intros * ? [IHA] ? [IHB] **.
@@ -496,7 +510,7 @@ Proof.
     simp conv conv_tm_red ; cbn.
     econstructor.
     1: exact IHA.
-    econstructor.
+    cbn; patch_rec_ret; econstructor.
     1: exact IHB.
     now constructor.
   - intros * ??? [ihFst] ? [ihSnd] **.
@@ -504,7 +518,7 @@ Proof.
     simp conv conv_tm_red ; cbn.
     econstructor.
     1: exact ihFst.
-    econstructor.
+    cbn; patch_rec_ret; econstructor.
     1: exact ihSnd.
     now constructor.
   - intros * ? [IHm []] wP **.
